More consistent naming
Predicates are now uppercase, everything else lowercase. Lemma names
which contain other entities' names use consistent capitalisation.

src/Equiv.v
@@ -1,36 +1,36 @@
 Require Import Env Sty Shape Subst Tac Var.
 
-Inductive sequiv_gen sequiv : Sty -> Sty -> Prop :=
-| sequiv_gen_end : sequiv_gen sequiv unit unit
-| sequiv_gen_send : forall B S S',
-    sequiv S S' ->
-    sequiv_gen sequiv (send B S) (send B S')
-| sequiv_gen_recv : forall B S S',
-    sequiv S S' ->
-    sequiv_gen sequiv (recv B S) (recv B S')
-| sequiv_gen_echoice : forall S1 S2 S1' S2',
-    sequiv S1 S1' ->
-    sequiv S2 S2' ->
-    sequiv_gen sequiv (echoice S1 S2) (echoice S1' S2')
-| sequiv_gen_ichoice : forall S1 S2 S1' S2',
-    sequiv S1 S1' ->
-    sequiv S2 S2' ->
-    sequiv_gen sequiv (ichoice S1 S2) (ichoice S1' S2')
-| sequiv_gen_mu1 : forall X S S',
-    sequiv (subst X (mu X S) S) S' ->
-    sequiv_gen sequiv (mu X S) S'
-| sequiv_gen_mu2 : forall X S S',
-    sequiv S (subst X (mu X S') S') ->
-    sequiv_gen sequiv S (mu X S')
+Inductive Sequiv_gen Sequiv : Sty -> Sty -> Prop :=
+| Sequiv_gen_end : Sequiv_gen Sequiv unit unit
+| Sequiv_gen_send : forall B S S',
+    Sequiv S S' ->
+    Sequiv_gen Sequiv (send B S) (send B S')
+| Sequiv_gen_recv : forall B S S',
+    Sequiv S S' ->
+    Sequiv_gen Sequiv (recv B S) (recv B S')
+| Sequiv_gen_echoice : forall S1 S2 S1' S2',
+    Sequiv S1 S1' ->
+    Sequiv S2 S2' ->
+    Sequiv_gen Sequiv (echoice S1 S2) (echoice S1' S2')
+| Sequiv_gen_ichoice : forall S1 S2 S1' S2',
+    Sequiv S1 S1' ->
+    Sequiv S2 S2' ->
+    Sequiv_gen Sequiv (ichoice S1 S2) (ichoice S1' S2')
+| Sequiv_gen_mu1 : forall X S S',
+    Sequiv (subst X (mu X S) S) S' ->
+    Sequiv_gen Sequiv (mu X S) S'
+| Sequiv_gen_mu2 : forall X S S',
+    Sequiv S (subst X (mu X S') S') ->
+    Sequiv_gen Sequiv S (mu X S')
 .
-Hint Constructors sequiv_gen.
+Hint Constructors Sequiv_gen.
 
-CoInductive sequiv : Sty -> Sty -> Prop :=
-| sequiv_fold : forall S S', sequiv_gen sequiv S S' -> sequiv S S'.
-Hint Constructors sequiv.
+CoInductive Sequiv : Sty -> Sty -> Prop :=
+| Sequiv_fold : forall S S', Sequiv_gen Sequiv S S' -> Sequiv S S'.
+Hint Constructors Sequiv.
 
 
-Lemma sequiv_coind : forall R,
-  (forall S S', R S S' -> sequiv_gen R S S')
-  -> (forall S S', R S S' -> sequiv S S').
+Lemma Sequiv_coind : forall R,
+  (forall S S', R S S' -> Sequiv_gen R S S')
+  -> (forall S S', R S S' -> Sequiv S S').
 Proof. cofix CIH. introv H HR. apply H in HR. inverts HR; eauto. Qed.
