src/NonEquiv.v
@@ -2,52 +2,52 @@ Require Import Sty Subst Shape Msg Var.
 
 Create HintDb nsequiv discriminated.
 
-Inductive nsequiv : Sty -> Sty -> Prop :=
-| nsequiv_send_S :
+Inductive NSequiv : Sty -> Sty -> Prop :=
+| NSequiv_send_S :
     forall B S S',
-    nsequiv S S' ->
-    nsequiv (send B S) (send B S')
-| nsequiv_send_B :
+    NSequiv S S' ->
+    NSequiv (send B S) (send B S')
+| NSequiv_send_B :
     forall B B' S S',
     B <> B' ->
-    nsequiv (send B S) (send B' S')
-| nsequiv_recv_S :
+    NSequiv (send B S) (send B' S')
+| NSequiv_recv_S :
     forall B S S',
-    nsequiv S S' ->
-    nsequiv (recv B S) (recv B S')
-| nsequiv_recv_B :
+    NSequiv S S' ->
+    NSequiv (recv B S) (recv B S')
+| NSequiv_recv_B :
     forall B B' S S',
     B <> B' ->
-    nsequiv (recv B S) (recv B' S')
-| nsequiv_echoice_l :
+    NSequiv (recv B S) (recv B' S')
+| NSequiv_echoice_l :
     forall S1 S2 S1' S2',
-    nsequiv S1 S1' ->
-    nsequiv (echoice S1 S2) (echoice S1' S2')
-| nsequiv_echoice_r :
+    NSequiv S1 S1' ->
+    NSequiv (echoice S1 S2) (echoice S1' S2')
+| NSequiv_echoice_r :
     forall S1 S2 S1' S2',
-    nsequiv S2 S2' ->
-    nsequiv (echoice S1 S2) (echoice S1' S2')
-| nsequiv_ichoice_l :
+    NSequiv S2 S2' ->
+    NSequiv (echoice S1 S2) (echoice S1' S2')
+| NSequiv_ichoice_l :
     forall S1 S2 S1' S2',
-    nsequiv S1 S1' ->
-    nsequiv (ichoice S1 S2) (ichoice S1' S2')
-| nsequiv_ichoice_r :
+    NSequiv S1 S1' ->
+    NSequiv (ichoice S1 S2) (ichoice S1' S2')
+| NSequiv_ichoice_r :
     forall S1 S2 S1' S2',
-    nsequiv S2 S2' ->
-    nsequiv (ichoice S1 S2) (ichoice S1' S2')
-| nsequiv_mu_l :
+    NSequiv S2 S2' ->
+    NSequiv (ichoice S1 S2) (ichoice S1' S2')
+| NSequiv_mu_l :
     forall X S S',
-    nsequiv (subst X (mu X S) S) S' ->
-    nsequiv (mu X S) S'
-| nsequiv_mu_r :
+    NSequiv (subst X (mu X S) S) S' ->
+    NSequiv (mu X S) S'
+| NSequiv_mu_r :
     forall X S S',
-    nsequiv S (subst X (mu X S') S') ->
-    nsequiv S (mu X S')
-| nsequiv_shape :
+    NSequiv S (subst X (mu X S') S') ->
+    NSequiv S (mu X S')
+| NSequiv_shape :
     forall S S',
     shape S  <> muS ->
     shape S' <> muS ->
     shape S <> shape S' ->
-    nsequiv S S'
+    NSequiv S S'
 .
-Hint Constructors nsequiv : nsequiv.
+Hint Constructors NSequiv : nsequiv.
