src/Reflexivity.v
@@ -5,29 +5,29 @@ Create HintDb refl discriminated.
 Inductive R_refl : Sty -> Sty -> Prop :=
 | refl_helper_refl :
     forall S,
-    wellformed S ->
+    Wf S ->
     R_refl S S
 | refl_helper_mu1   :
     forall X S,
-    wellformed (subst X (mu X S) S) ->
+    Wf (subst X (mu X S) S) ->
     R_refl (mu X S) (subst X (mu X S) S)
 | refl_helper_mu2 :
     forall X S,
-    wellformed (subst X (mu X S) S) ->
+    Wf (subst X (mu X S) S) ->
     R_refl (subst X (mu X S) S) (mu X S)
 .
 Hint Constructors R_refl : refl.
 
 Lemma R_refl_reflexivity :
-  (forall S S', R_refl S S' -> sequiv S S')
-  -> (forall S, wellformed S -> sequiv S S).
+  (forall S S', R_refl S S' -> Sequiv S S')
+  -> (forall S, Wf S -> Sequiv S S).
 Proof. auto with refl. Qed.
 
-Theorem sequiv_reflexive :
+Theorem Sequiv_reflexive :
   forall S,
-  wellformed S ->
-  sequiv S S.
+  Wf S ->
+  Sequiv S S.
 Proof.
-  apply R_refl_reflexivity. apply sequiv_coind.
+  apply R_refl_reflexivity. apply Sequiv_coind.
   introv H. inverts1 H; [destruct S'|..]; auto with wf refl.
 Qed.
