src/Transitivity.v
@@ -2,65 +2,65 @@ Require Import CS CSFacts Equiv Reflexivity Sty StyInd Subst SubstFacts Tac Wf
   WfFacts.
 
 Create HintDb trans discriminated.
-Hint Resolve sequiv_reflexive : trans.
+Hint Resolve Sequiv_reflexive : trans.
 
 
 Inductive trans_helper : Sty -> Sty -> Prop :=
 | trans_helper_trans :
     forall S T U,
-    wellformed S ->
-    wellformed T ->
-    wellformed U ->
-    sequiv S T ->
-    sequiv T U ->
+    Wf S ->
+    Wf T ->
+    Wf U ->
+    Sequiv S T ->
+    Sequiv T U ->
     trans_helper S U
 .
 Hint Constructors trans_helper : trans.
 
 Lemma trans_helper_refl :
   forall S,
-  wellformed S ->
+  Wf S ->
   trans_helper S S.
 Proof. eauto with trans. Qed.
 
-Lemma sequiv_impl_trans_helper :
+Lemma Sequiv_impl_trans_helper :
   forall S T,
-  wellformed S ->
-  wellformed T ->
-  sequiv S T ->
+  Wf S ->
+  Wf T ->
+  Sequiv S T ->
   trans_helper S T.
 Proof. eauto with trans. Qed.
 
 Lemma trans_helper_transitive :
-  (forall S T, trans_helper S T -> sequiv S T) ->
+  (forall S T, trans_helper S T -> Sequiv S T) ->
   (forall S T U,
-    wellformed S ->
-    wellformed T ->
-    wellformed U ->
-    sequiv S T ->
-    sequiv T U ->
-    sequiv S U
+    Wf S ->
+    Wf T ->
+    Wf U ->
+    Sequiv S T ->
+    Sequiv T U ->
+    Sequiv S U
   ).
 Proof. eauto with trans. Qed.
 
 
 (* TODO beautify (a lot) *)
-Theorem sequiv_transitive :
+Theorem Sequiv_transitive :
   forall S T U,
-  wellformed S ->
-  wellformed T ->
-  wellformed U ->
-  sequiv S T ->
-  sequiv T U ->
-  sequiv S U.
+  Wf S ->
+  Wf T ->
+  Wf U ->
+  Sequiv S T ->
+  Sequiv T U ->
+  Sequiv S U.
 Proof.
-  apply trans_helper_transitive. apply sequiv_coind.
+  apply trans_helper_transitive. apply Sequiv_coind.
   introv H. rename S' into U. inverts H.
-  assert (sequiv S (cs T)) as HSeqT  by (
-    eapply cs_preserves_sequiv_r; eauto with wf
+  assert (Sequiv S (cs T)) as HSeqT  by (
+    eapply cs_preserves_Sequiv_r; eauto with wf
   ).
-  assert (sequiv (cs T) U) as HTeqU by (
-    eapply cs_preserves_sequiv_l; eauto with wf
+  assert (Sequiv (cs T) U) as HTeqU by (
+    eapply cs_preserves_Sequiv_l; eauto with wf
   ).
   clear H3 H4. inverts2 HSeqT; inverts2 HTeqU; subst; try solve [false].
 
@@ -68,12 +68,12 @@ Proof.
   - auto.
 
   - constructor. rewrite <- HSeqT in *.
-    apply sequiv_impl_trans_helper; auto with wf.
+    apply Sequiv_impl_trans_helper; auto with wf.
 
   (* send *)
   - rewrite <- H4 in H3. injection H3; intros; subst.
     constructor. apply trans_helper_trans with (T := S); eauto with wf.
-      apply cs_preserves_wellformed in H1. rewrite <- H4 in H1.
+      apply cs_preserves_Wf in H1. rewrite <- H4 in H1.
       eauto with wf.
 
   - constructor. rewrite <- H3 in *.
@@ -83,7 +83,7 @@ Proof.
   (* recv *)
   - rewrite <- H4 in H3. injection H3; intros; subst.
     constructor. apply trans_helper_trans with (T := S); eauto with wf.
-      apply cs_preserves_wellformed in H1. rewrite <- H4 in H1.
+      apply cs_preserves_Wf in H1. rewrite <- H4 in H1.
       eauto with wf.
 
   - constructor. rewrite <- H3 in *.
@@ -91,29 +91,29 @@ Proof.
       rewrite H3. eauto with wf.
 
   (* echoice *)
-  - assert (wellformed (echoice S1' S2')) by (rewrite H3; eauto with wf).
+  - assert (Wf (echoice S1' S2')) by (rewrite H3; eauto with wf).
     rewrite <- H4 in H3. injection H3; intros; subst.
     constructor.
     * apply trans_helper_trans with (T := S0); eauto with wf.
     * apply trans_helper_trans with (T := S3); eauto with wf.
 
-  - assert (wellformed (echoice S1' S2')) by (rewrite H3; eauto with wf).
+  - assert (Wf (echoice S1' S2')) by (rewrite H3; eauto with wf).
     constructor. rewrite <- H3 in *.
     apply trans_helper_trans with (T := echoice S1' S2'); eauto with wf.
 
   (* ichoice *)
-  - assert (wellformed (ichoice S1' S2')) by (rewrite H3; eauto with wf).
+  - assert (Wf (ichoice S1' S2')) by (rewrite H3; eauto with wf).
     rewrite <- H4 in H3. injection H3; intros; subst.
     constructor.
     * apply trans_helper_trans with (T := S0); eauto with wf.
     * apply trans_helper_trans with (T := S3); eauto with wf.
 
-  - assert (wellformed (ichoice S1' S2')) by (rewrite H3; eauto with wf).
+  - assert (Wf (ichoice S1' S2')) by (rewrite H3; eauto with wf).
     constructor. rewrite <- H3 in *.
     apply trans_helper_trans with (T := ichoice S1' S2'); eauto with wf.
 
   (* unit *)
-  - rewrite <- HTeqU in *. constructor. apply sequiv_impl_trans_helper;
+  - rewrite <- HTeqU in *. constructor. apply Sequiv_impl_trans_helper;
       auto with wf.
 
   (* send *)
@@ -141,7 +141,7 @@ Proof.
 
   (* mu 2 *)
   - constructor.
-    assert (sequiv (cs T) (mu X0 S')) as HTeqU' by auto.
+    assert (Sequiv (cs T) (mu X0 S')) as HTeqU' by auto.
     apply trans_helper_trans with (T := cs T);
       eauto with wf.
 
