src/TraceBisimEquiv.v
@@ -5,18 +5,18 @@ Require Import Contractive CS CSFacts Equiv Free Sty Subst SubstFacts Msg Tac
 Inductive R_trace_bisim_equivalence' : Sty -> Sty -> Prop :=
 | R_trace_bisim_equivalence'_intro :
     forall S S' eta c c',
-    wellformed S ->
-    wellformed S' ->
+    Wf S ->
+    Wf S' ->
     Tl_bisim (tl eta S c) (tl eta S' c') ->
     R_trace_bisim_equivalence' S S'.
 
 
 Lemma trace_bisim_equivalence' :
   forall S S' eta c c',
-  wellformed S ->
-  wellformed S' ->
+  Wf S ->
+  Wf S' ->
   Tl_bisim (tl eta S c) (tl eta S' c') ->
-  sequiv S S'.
+  Sequiv S S'.
 Proof.
   Ltac solve_same_shape H :=
     inverts2 H; constructor; econstructor; eauto with wf
@@ -26,18 +26,18 @@ Proof.
     erewrite tl_mu_subst in H; [constructor; econstructor|]; eauto with free wf
   .
 
-  Ltac solve_wellformed_var :=
+  Ltac solve_Wf_var :=
     match goal with
-    | _ : wellformed (var _) |- _ => auto with wf
+    | _ : Wf (var _) |- _ => auto with wf
     end
   .
 
-  intros. apply sequiv_coind with (R := R_trace_bisim_equivalence');
+  intros. apply Sequiv_coind with (R := R_trace_bisim_equivalence');
     [|econstructor; eauto].
   clear. introv H. inverts H. rename H2 into Heq. destruct S; destruct S';
     try solve
       [ constructor
-      | solve_wellformed_var
+      | solve_Wf_var
       | solve_mu Heq
       | solve_same_shape Heq
       ].
@@ -47,21 +47,21 @@ Qed.
 
 Theorem trace_bisim_equivalence :
   forall S S' eta
-  (Swf : wellformed S)
-  (Swf' : wellformed S'),
+  (Swf : Wf S)
+  (Swf' : Wf S'),
   Tl_bisim
-    (tl eta S (wellformed_Contractive Swf))
-    (tl eta S' (wellformed_Contractive Swf')) ->
-  sequiv S S'.
+    (tl eta S (Wf_Contractive Swf))
+    (tl eta S' (Wf_Contractive Swf')) ->
+  Sequiv S S'.
 Proof. intros. eapply trace_bisim_equivalence'; eauto. Qed.
 
 Theorem trace_eq_equivalence :
   forall S S' eta
-  (Swf : wellformed S)
-  (Swf' : wellformed S'),
-  (tl eta S (wellformed_Contractive Swf)) =
-    (tl eta S' (wellformed_Contractive Swf')) ->
-  sequiv S S'.
+  (Swf : Wf S)
+  (Swf' : Wf S'),
+  (tl eta S (Wf_Contractive Swf)) =
+    (tl eta S' (Wf_Contractive Swf')) ->
+  Sequiv S S'.
 Proof. introv H. eapply trace_bisim_equivalence. rewrite H. reflexivity. Qed.
 
 
@@ -71,9 +71,9 @@ Inductive R_equivalence_trace_bisim' : Tl -> Tl -> Prop :=
     (exists S S' c c',
      tl eta (cs S) c = l /\
      tl eta (cs S') c' = l' /\
-     wellformed S /\
-     wellformed S' /\
-     sequiv (cs S) (cs S')
+     Wf S /\
+     Wf S' /\
+     Sequiv (cs S) (cs S')
     ) ->
     R_equivalence_trace_bisim' l l'
 .
@@ -82,25 +82,25 @@ Inductive R_equivalence_trace_bisim' : Tl -> Tl -> Prop :=
 (* TODO ouch *)
 Lemma equivalence_trace_bisim' :
   forall S S' eta c c',
-  wellformed S ->
-  wellformed S' ->
-  sequiv S S' ->
+  Wf S ->
+  Wf S' ->
+  Sequiv S S' ->
   Tl_bisim (tl eta S c) (tl eta S' c').
 Proof.
   Ltac wf_inv S1 H1 S2 :=
     let Htmp := fresh in
-    assert (wellformed S1) as Htmp by (rewrite H1; auto with wf);
-    assert (wellformed S2) by (auto with wf);
+    assert (Wf S1) as Htmp by (rewrite H1; auto with wf);
+    assert (Wf S2) by (auto with wf);
     clear Htmp
   .
 
   intros. (rewrite_strat (subterms cs_preserves_tl)); try assumption.
   apply Tl_bisim_coind with (R := R_equivalence_trace_bisim').
   - clear. introv CIH. inverts1 CIH. norm_hyp_auto.
-    rename H0 into Hwf. rename H2 into Hwf'. rename H4 into Hsequiv.
-    subst. inverts2 Hsequiv.
-    * gen c c' Hwf Hwf'. rewrite <- Hsequiv. rewrite <- H2.
-      clear Hsequiv. intros. constructor.
+    rename H0 into Hwf. rename H2 into Hwf'. rename H4 into HSequiv.
+    subst. inverts2 HSequiv.
+    * gen c c' Hwf Hwf'. rewrite <- HSequiv. rewrite <- H2.
+      clear HSequiv. intros. constructor.
     * gen c c' Hwf Hwf'. rewrite <- H0. rewrite <- H1.
       introv Hwf Hwf'.
       wf_inv (send B S0) H0 S0.
@@ -111,7 +111,7 @@ Proof.
       + symmetry. apply cs_preserves_tl. assumption.
       + assumption.
       + assumption.
-      + apply cs_preserves_sequiv; eauto with wf.
+      + apply cs_preserves_Sequiv; eauto with wf.
     * gen c c' Hwf Hwf'. rewrite <- H0. rewrite <- H1.
       introv Hwf Hwf'.
       wf_inv (recv B S0) H0 S0.
@@ -122,7 +122,7 @@ Proof.
       + symmetry. apply cs_preserves_tl. assumption.
       + assumption.
       + assumption.
-      + apply cs_preserves_sequiv; eauto with wf.
+      + apply cs_preserves_Sequiv; eauto with wf.
     * gen c c' Hwf Hwf'. rewrite <- H0. rewrite <- H1.
       introv Hwf Hwf'.
       wf_inv (echoice S1 S2) H0 S1.
@@ -135,13 +135,13 @@ Proof.
         -- symmetry. apply cs_preserves_tl. assumption.
         -- assumption.
         -- assumption.
-        -- apply cs_preserves_sequiv; eauto with wf.
+        -- apply cs_preserves_Sequiv; eauto with wf.
       + econstructor. exists S2. exists S2'. eexists. eexists. splits.
         -- symmetry. apply cs_preserves_tl. assumption.
         -- symmetry. apply cs_preserves_tl. assumption.
         -- assumption.
         -- assumption.
-        -- apply cs_preserves_sequiv; eauto with wf.
+        -- apply cs_preserves_Sequiv; eauto with wf.
     * gen c c' Hwf Hwf'. rewrite <- H0. rewrite <- H1.
       introv Hwf Hwf'.
       wf_inv (ichoice S1 S2) H0 S1.
@@ -154,13 +154,13 @@ Proof.
         -- symmetry. apply cs_preserves_tl. assumption.
         -- assumption.
         -- assumption.
-        -- apply cs_preserves_sequiv; eauto with wf.
+        -- apply cs_preserves_Sequiv; eauto with wf.
       + econstructor. exists S2. exists S2'. eexists. eexists. splits.
         -- symmetry. apply cs_preserves_tl. assumption.
         -- symmetry. apply cs_preserves_tl. assumption.
         -- assumption.
         -- assumption.
-        -- apply cs_preserves_sequiv; eauto with wf.
+        -- apply cs_preserves_Sequiv; eauto with wf.
     * symmetry in H0. apply cs_mu_absurd in H0.
       + contradiction.
       + eauto with contractive wf.
@@ -169,16 +169,16 @@ Proof.
       + eauto with contractive wf.
   - econstructor. exists S. exists S'. eexists. eexists. splits;
     auto with subst.
-    * apply cs_preserves_sequiv; assumption.
+    * apply cs_preserves_Sequiv; assumption.
 Unshelve.
   all: auto with wf.
 Qed.
 
 Theorem equivalence_trace_bisim :
   forall S S' eta
-  (Swf : wellformed S)
-  (S'wf : wellformed S'),
-  sequiv S S' ->
-  Tl_bisim (tl eta S (wellformed_Contractive Swf))
-    (tl eta S' (wellformed_Contractive S'wf)).
+  (Swf : Wf S)
+  (S'wf : Wf S'),
+  Sequiv S S' ->
+  Tl_bisim (tl eta S (Wf_Contractive Swf))
+    (tl eta S' (Wf_Contractive S'wf)).
 Proof. intros. apply equivalence_trace_bisim'; auto. Qed.
