src/WfFacts.v
@@ -2,36 +2,36 @@ Require Import Contractive ContractiveFacts CSFacts Free FreeFacts SubstFacts
   Sty Tac Wf.
 
 
-Hint Resolve cs_preserves_wellformed : wf.
-Hint Resolve wellformed_Contractive : wf.
-Hint Resolve wellformed_Closed : wf.
-Hint Resolve mu_unfold_preserves_wellformed : wf.
+Hint Resolve cs_preserves_Wf : wf.
+Hint Resolve Wf_Contractive : wf.
+Hint Resolve Wf_Closed : wf.
+Hint Resolve mu_unfold_preserves_Wf : wf.
 
 
-Lemma wellformed_inv :
+Lemma Wf_inv :
   forall S S',
   StySubSimple S S' ->
-  wellformed S' ->
-  wellformed S.
+  Wf S' ->
+  Wf S.
 Proof.
-  introv sub; inverts1 sub; unfold wellformed in *;
+  introv sub; inverts1 sub; unfold Wf in *;
   auto with contractive free.
 Qed.
 
 
-Hint Extern 2 (wellformed ?S) =>
+Hint Extern 2 (Wf ?S) =>
   match goal with
-  | H : wellformed _ |- _ =>
-      solve [apply (wellformed_inv S) in H; [exact H | auto with stysub]]
+  | H : Wf _ |- _ =>
+      solve [apply (Wf_inv S) in H; [exact H | auto with stysub]]
   end
 : wf.
 
 
 Hint Extern 2 =>
   match goal with
-  | H : wellformed (var _) |- _ =>
+  | H : Wf (var _) |- _ =>
       solve [
-        unfold wellformed in H; destruct H as [_ H]; apply Closed_var_absurd in H;
+        unfold Wf in H; destruct H as [_ H]; apply Closed_var_absurd in H;
         contradiction
       ]
   end
